reduce from three to two invariants for NAND

NAND_Hoare.thy
@@ -20,16 +20,7 @@ definition nand_inv :: "sig assn2" where
   "nand_inv \<equiv> (\<lambda>tw. \<forall>i < fst tw. snd tw C (i + 1) \<longleftrightarrow> \<not> (snd tw A i \<and> snd tw B i))"
 
 definition nand_inv2 :: "sig assn2" where
-  "nand_inv2 \<equiv> (\<lambda>tw. C \<in> event_of tw \<longrightarrow> (\<forall>i> fst tw. snd tw C i = snd tw C (fst tw)))"
-
-definition nand_inv3 :: "sig assn2" where
-  "nand_inv3 \<equiv> (\<lambda>tw. event_of tw = {} \<longrightarrow> (snd tw C (fst tw + 1) \<longleftrightarrow> \<not> (snd tw A (fst tw) \<and> snd tw B (fst tw)))
-                                       \<and>  (\<forall>i> fst tw + 1. snd tw C i = snd tw C (fst tw + 1)))"
-
-lemma nand_seq_hoare:
-  "\<turnstile> [nand_inv] (Bassign_trans C (Bnand (Bsig A) (Bsig B)) 1) [nand_inv]"
-  by (rule Conseq2[where Q="nand_inv", rotated 1], rule Assign2)
-     (auto simp add :worldline_upd2_def worldline_upd_def nand_inv_def)
+  "nand_inv2 \<equiv> (\<lambda>tw. disjnt {A, B} (event_of tw) \<longrightarrow> (\<forall>i\<ge>fst tw. snd tw C (i + 1) \<longleftrightarrow> \<not> (snd tw A (fst tw) \<and> snd tw B (fst tw))))"
 
 lemma nand_inv_next_time:
   assumes "nand_inv tw"
@@ -114,425 +105,199 @@ lemma nand_seq_hoare_next_time0:
   apply (rule Conseq2[where Q="\<lambda>tw. nand_inv (next_time_world tw, snd tw)", rotated 1], rule Assign2)
   using nand_inv_next_time0 by auto
 
+lemma disjnt_AB_eq:
+  "disjnt {A, B} s \<longleftrightarrow> (s = {} \<or> s = {C})"
+  by (rule, metis Diff_UNIV Diff_insert0 Diff_single_insert UNIV_sig disjnt_insert1 empty_subsetI
+  subset_singleton_iff) auto
+
+lemma nand_conc_hoare':
+  "\<And>tw. nand_inv tw \<and> nand_inv2 tw \<and> disjnt {A, B} (event_of tw) \<Longrightarrow> nand_inv (next_time_world tw, snd tw)"
+proof -
+  fix tw
+  assume "nand_inv tw \<and> nand_inv2 tw \<and> disjnt {A, B} (event_of tw)"
+  hence "nand_inv tw" and "nand_inv2 tw" and "disjnt {A, B} (event_of tw)"
+    by auto
+  hence *: "\<forall>i < fst tw. snd tw C (i + 1) \<longleftrightarrow> \<not> (snd tw A i \<and> snd tw B i)"
+    unfolding nand_inv_def by auto
+  have **: "\<forall>i\<ge>fst tw. i < next_time_world tw \<longrightarrow> (\<forall>s. snd tw s i = snd tw s (fst tw))"
+    using unchanged_until_next_time_world by blast
+  have ***: "(\<forall>i\<ge> fst tw. snd tw C (i + 1) \<longleftrightarrow> \<not> (snd tw A (fst tw) \<and>  snd tw B (fst tw)))"
+    using \<open>nand_inv2 tw\<close> \<open>disjnt {A, B} (event_of tw)\<close> unfolding nand_inv2_def by auto
+
+  \<comment> \<open>obtain the value of A and B at time fst tw\<close>
+  have "snd tw A (fst tw) = snd tw A (fst tw - 1)" and "snd tw B (fst tw) = snd tw B (fst tw - 1)"
+    using \<open>disjnt {A, B} (event_of tw)\<close> unfolding event_of_alt_def 
+    by (smt diff_0_eq_0 disjnt_insert1 mem_Collect_eq)+
+ { fix i 
+    assume "i < next_time_world tw"
+    have "i < fst tw \<or> fst tw \<le> i" 
+      by auto
+    moreover
+    { assume "i < fst tw"
+      hence "snd tw C (i + 1) \<longleftrightarrow> \<not> (snd tw A i \<and> snd tw B i)"
+        using * by auto }
+    moreover
+    { assume "fst tw \<le> i"
+      hence "snd tw C (i + 1) \<longleftrightarrow> snd tw C (fst tw + 1)"
+        using *** by auto
+      also have "... \<longleftrightarrow> \<not> (snd tw A (fst tw) \<and> snd tw B (fst tw))"
+        using *** \<open>fst tw \<le> i\<close> by auto
+      also have "... \<longleftrightarrow> \<not> (snd tw A i \<and> snd tw B i)"
+        using ** \<open>i < next_time_world tw\<close> \<open>fst tw \<le> i\<close> less_imp_le_nat by blast
+      finally have "snd tw C (i + 1) \<longleftrightarrow> \<not> (snd tw A i \<and> snd tw B i)"
+        by auto }
+    ultimately have "snd tw C (i + 1) \<longleftrightarrow> \<not> (snd tw A i \<and> snd tw B i)"
+      by auto }
+  hence "\<And>i. i < next_time_world tw \<Longrightarrow> snd tw C (i + 1) \<longleftrightarrow> \<not> (snd tw A i \<and> snd tw B i)"
+    by auto
+  thus "nand_inv (next_time_world tw, snd tw)"
+    unfolding nand_inv_def by auto
+qed
+
+lemma nand_conc_hoare2: 
+  "\<And>tw. nand_inv tw \<and> nand_inv2 tw \<and> disjnt {A, B} (event_of tw) \<Longrightarrow> nand_inv2 (next_time_world tw, snd tw)"
+proof -
+  fix tw
+  assume "nand_inv tw \<and> nand_inv2 tw \<and> disjnt {A, B} (event_of tw)"
+  hence "nand_inv tw" and "nand_inv2 tw" and "disjnt {A, B} (event_of tw)"
+    by auto
+  hence 0: "(\<forall>i\<ge>fst tw. snd tw C (i + 1) = (\<not> (snd tw A (fst tw) \<and> snd tw B (fst tw))))"
+    unfolding nand_inv2_def by auto  
+  have 1: "\<forall>i\<ge>fst tw. i < next_time_world tw \<longrightarrow> (\<forall>s. snd tw s i = snd tw s (fst tw))"
+    using unchanged_until_next_time_world by blast
+  let ?t' = "next_time_world tw"
+  { assume "disjnt {A, B} (event_of (next_time_world tw, snd tw))" 
+    hence *: "snd tw A ?t' = snd tw A (?t' - 1)" and **: "snd tw B ?t' = snd tw B (?t' - 1)"
+      unfolding event_of_alt_def  by (smt diff_0_eq_0 disjnt_insert1 fst_conv mem_Collect_eq snd_conv)+
+    have "fst tw < next_time_world tw"
+      by (simp add: next_time_world_at_least)
+    { fix i
+      assume "?t' \<le> i"
+      hence "snd tw C (i + 1) \<longleftrightarrow> \<not> (snd tw A (fst tw) \<and> snd tw B (fst tw))"
+        using 0 \<open>fst tw < ?t'\<close> by auto
+      moreover have "snd tw A (fst tw) = snd tw A (?t' - 1)" and "snd tw B (fst tw) = snd tw B (?t' - 1)"
+        using 1 
+        by (metis (no_types, lifting) One_nat_def Suc_leI \<open>get_time tw < next_time_world tw\<close>
+        add_le_cancel_right diff_add diff_less discrete gr_implies_not_zero neq0_conv zero_less_one)+
+      ultimately have "snd tw C (i + 1) \<longleftrightarrow> \<not> (snd tw A ?t' \<and> snd tw B ?t')"
+        using * ** by auto
+    }
+    hence "(\<forall>i\<ge>?t'. snd tw C (i + 1) = (\<not> (snd tw A ?t' \<and> snd tw B ?t')))"
+      by auto }
+  thus "nand_inv2 (next_time_world tw, snd tw)"
+    unfolding nand_inv2_def by auto
+qed
+
 lemma nand_inv2_next_time:
   fixes tw
   defines "tw' \<equiv> tw[C, 1 :=\<^sub>2 beval_world_raw2 tw (Bnand (Bsig A) (Bsig B))]"
   shows   "nand_inv2 (next_time_world tw', snd tw')"
   unfolding nand_inv2_def
 proof (rule impI)
-  assume "C \<in> event_of (next_time_world tw', snd tw')"
-  have "0 < next_time_world tw"
-    using next_time_world_at_least gr_implies_not_zero by blast
-  hence "event_of (next_time_world tw', snd tw') = {s. snd tw' s (next_time_world tw') \<noteq> snd tw' s (next_time_world tw' - 1)}"
-    unfolding event_of_alt_def by (metis fst_conv next_time_world_at_least not_less0 snd_conv)
-  hence "snd tw' C (next_time_world tw') \<noteq> snd tw' C (next_time_world tw' - 1)"
-    using \<open>C \<in> event_of (next_time_world tw', snd tw')\<close> by auto
-  have "next_time_world tw' = fst tw + 1"
-  proof (rule ccontr)
-    assume "next_time_world tw' \<noteq> fst tw + 1"
-    hence "next_time_world tw' < fst tw + 1 \<or> next_time_world tw' > fst tw + 1" 
-      by auto
-    moreover
-    { assume "next_time_world tw' < fst tw + 1"
-      hence "False"
-        using next_time_world_at_least 
-        by (metis assms(1) discrete fstI leD worldline_upd2_def) }
-    moreover
-    { assume "fst tw + 1 < next_time_world tw'"
-      hence False
-        by (smt One_nat_def Suc_diff_1 Suc_eq_plus1 \<open>snd tw' C (next_time_world tw') \<noteq> snd tw' C
-        (next_time_world tw' - 1)\<close> assms(1) calculation(2) discrete dual_order.strict_trans leD
-        le_add2 snd_conv worldline_upd2_def worldline_upd_def) }
-    ultimately show False 
-      by auto
+  assume "disjnt {A, B} (event_of (next_time_world tw', snd tw'))"
+  let ?t' = "next_time_world tw'"
+  have "fst tw' < ?t'"
+    using next_time_world_at_least by blast
+  moreover have "fst tw = fst tw'"
+    unfolding tw'_def unfolding worldline_upd2_def by auto
+  ultimately have "fst tw < ?t'"
+    by auto
+  have "snd tw' A ?t' \<longleftrightarrow> snd tw A ?t'"
+    unfolding tw'_def worldline_upd2_def worldline_upd_def by auto
+  also have "... \<longleftrightarrow> snd tw A (?t' - 1)"
+    using \<open>disjnt {A, B} (event_of (next_time_world tw', snd tw'))\<close> \<open>fst tw < ?t'\<close>
+    unfolding event_of_alt_def 
+    by (simp add: tw'_def worldline_upd2_def worldline_upd_def)
+  also have "... \<longleftrightarrow> snd tw A (fst tw)"
+  proof -
+    have "fst tw' \<le> ?t' - 1" and "?t' - 1 < ?t'"
+      using \<open>fst tw' < ?t'\<close> by auto
+    hence "snd tw' A (?t' - 1) = snd tw' A (fst tw')"
+      using unchanged_until_next_time_world[where tw="tw'"] by blast
+    moreover have "snd tw' A (?t' - 1) = snd tw A (?t' - 1)"
+      unfolding tw'_def worldline_upd2_def worldline_upd_def by auto
+    moreover have "snd tw' A (fst tw') = snd tw A (fst tw')"
+      unfolding tw'_def worldline_upd2_def worldline_upd_def by auto
+    ultimately show ?thesis
+      using \<open>fst tw = fst tw'\<close> by auto
   qed
-  have "nand_inv2 (fst tw + 1, snd tw')"
-    using assms(1) unfolding tw'_def nand_inv2_def
-    by (simp add: worldline_upd2_def worldline_upd_def)
-  thus "\<forall>i>get_time (next_time_world tw', snd tw'). snd (next_time_world tw', snd tw') C i = 
-                      snd (next_time_world tw', snd tw') C (get_time (next_time_world tw', snd tw'))"
-    unfolding nand_inv2_def 
-    using \<open>C \<in> event_of (next_time_world tw', snd tw')\<close> \<open>next_time_world tw' = get_time tw + 1\<close> 
+  finally have 0: "snd tw' A ?t' \<longleftrightarrow> snd tw A (fst tw)"
+    by auto
+  have "snd tw' B ?t' \<longleftrightarrow> snd tw B ?t'"
+    unfolding tw'_def worldline_upd2_def worldline_upd_def by auto
+  also have "... \<longleftrightarrow> snd tw B (?t' - 1)"
+    using \<open>disjnt {A, B} (event_of (next_time_world tw', snd tw'))\<close> \<open>fst tw < ?t'\<close>
+    unfolding event_of_alt_def 
+    by (simp add: tw'_def worldline_upd2_def worldline_upd_def)
+  also have "... \<longleftrightarrow> snd tw B (fst tw)"
+  proof -
+    have "fst tw' \<le> ?t' - 1" and "?t' - 1 < ?t'"
+      using \<open>fst tw' < ?t'\<close> by auto
+    hence "snd tw' B (?t' - 1) = snd tw' B (fst tw')"
+      using unchanged_until_next_time_world[where tw="tw'"] by blast
+    moreover have "snd tw' B (?t' - 1) = snd tw B (?t' - 1)"
+      unfolding tw'_def worldline_upd2_def worldline_upd_def by auto
+    moreover have "snd tw' B (fst tw') = snd tw B (fst tw')"
+      unfolding tw'_def worldline_upd2_def worldline_upd_def by auto
+    ultimately show ?thesis
+      using \<open>fst tw = fst tw'\<close> by auto
+  qed
+  finally have 1: "snd tw' B ?t' \<longleftrightarrow> snd tw B (fst tw)"
+    by auto
+  { fix i 
+    assume "?t' \<le> i"
+    hence "snd tw' C (i + 1) \<longleftrightarrow> beval_world_raw2 tw (Bnand (Bsig A) (Bsig B))"
+      using `fst tw < ?t'`
+      unfolding tw'_def worldline_upd2_def worldline_upd_def by auto
+    also have "... \<longleftrightarrow> \<not> (snd tw A (fst tw) \<and> snd tw B (fst tw))"
+      unfolding beval_world_raw2_def beval_world_raw_def 
+      by (simp add: state_of_world_def)
+    also have "... \<longleftrightarrow> \<not> (snd tw' A ?t' \<and> snd tw' B ?t')"
+      using 0 1 by auto
+    finally have "snd tw' C (i + 1) \<longleftrightarrow> \<not> (snd tw' A ?t' \<and> snd tw' B ?t')"
+      by auto } 
+  thus "\<forall>i\<ge>get_time (next_time_world tw', snd tw').
+       snd (next_time_world tw', snd tw') C (i + 1) =
+       (\<not> (snd (next_time_world tw', snd tw') A (get_time (next_time_world tw', snd tw')) \<and>
+            snd (next_time_world tw', snd tw') B (get_time (next_time_world tw', snd tw'))))"
     by auto
 qed
 
-lemma nand_seq_hoare_next_time2:
-  "\<turnstile> [\<lambda>tw. True] (Bassign_trans C (Bnand (Bsig A) (Bsig B)) 1) [\<lambda>tw. nand_inv2 (next_time_world tw, snd tw)]"
+lemma nand_seq_hoare_next_time4:
+  " \<turnstile> [\<lambda>tw. True] Bassign_trans C (Bnand (Bsig A) (Bsig B)) 1 [\<lambda>tw. nand_inv2 (next_time_world tw, snd tw)]"
   apply (rule Conseq2[where Q="\<lambda>tw. nand_inv2 (next_time_world tw, snd tw)", rotated 1], rule Assign2)
   using nand_inv2_next_time by auto
-
-lemma nand_inv3_next_time:
-  fixes tw
-  defines "tw' \<equiv> tw[C, 1 :=\<^sub>2 beval_world_raw2 tw (Bnand (Bsig A) (Bsig B))]"
-  shows   "nand_inv3 (next_time_world tw', snd tw')"
-  unfolding nand_inv3_def
-proof (rule impI)
-  assume "event_of (next_time_world tw', snd tw') = {}"
-  have "0 < next_time_world tw"
-    using next_time_world_at_least gr_implies_not_zero by blast
-  hence "event_of (next_time_world tw', snd tw') = {s. snd tw' s (next_time_world tw') \<noteq> snd tw' s (next_time_world tw' - 1)}"
-    unfolding event_of_alt_def by (metis fst_conv next_time_world_at_least not_less0 snd_conv)
-  hence "\<And>s. snd tw' s (next_time_world tw') = snd tw' s (next_time_world tw' - 1)"
-    using \<open>event_of (next_time_world tw', snd tw') = {}\<close> by auto
-  hence *: "\<And>s. snd tw' s (next_time_world tw') = snd tw' s (fst tw')"
-    using unchanged_until_next_time_world 
-    by (smt diff_less discrete le_add2 le_less_trans less_diff_conv less_one next_time_world_at_least not_less)
-  have "next_time_world tw' = fst tw' + 1"
-  proof -
-    have "\<exists>n\<ge>get_time tw'. (\<lambda>s. snd tw' s (get_time tw')) \<noteq> (\<lambda>s. snd tw' s n) \<or> 
-          \<not> (\<exists>n\<ge>get_time tw'. (\<lambda>s. snd tw' s (get_time tw')) \<noteq> (\<lambda>s. snd tw' s n))"
-      by auto
-    moreover
-    { assume "\<not> (\<exists>n\<ge>get_time tw'. (\<lambda>s. snd tw' s (get_time tw')) \<noteq> (\<lambda>s. snd tw' s n))"
-      hence ?thesis
-        unfolding next_time_world_alt_def Let_def by auto }
-    moreover
-    { assume **: "\<exists>n\<ge>get_time tw'. (\<lambda>s. snd tw' s (get_time tw')) \<noteq> (\<lambda>s. snd tw' s n)"
-      hence "next_time_world tw' = (LEAST n. get_time tw' \<le> n \<and> (\<lambda>s. snd tw' s (get_time tw')) \<noteq> (\<lambda>s. snd tw' s n))"
-        unfolding next_time_world_alt_def Let_def by auto
-      hence "(\<lambda>s. snd tw' s (fst tw')) \<noteq> (\<lambda>s. snd tw' s (next_time_world tw'))"
-        using LeastI_ex[OF **] by auto
-      hence "\<exists>s. snd tw' s (fst tw') \<noteq> snd tw' s (next_time_world tw')"
-        by auto
-      with * have False by simp
-      hence ?thesis
-        by auto }
-    ultimately show ?thesis
-      by auto
-  qed
-  also have "... = fst tw + 1"
-    unfolding tw'_def  by (simp add: worldline_upd2_def)
-  finally have "next_time_world tw' = fst tw + 1"
-    by auto
-  have "snd tw' C (fst tw + 2) \<longleftrightarrow> \<not> (snd tw' A (fst tw + 1) \<and> snd tw' B (fst tw + 1))"
-  proof -
-    have "snd tw' C (fst tw + 2) \<longleftrightarrow> snd tw' C (fst tw + 1)"
-      unfolding tw'_def 
-      by (metis (no_types, hide_lams) BitM_plus_one Suc_eq_plus1 add_2_eq_Suc'
-      dual_order.strict_trans exp2_def lessI less_not_refl3 nat_less_le snd_conv worldline_upd2_def
-      worldline_upd_def)
-    have "snd tw' A (fst tw + 1) = snd tw' A (fst tw')" and  "snd tw' B (fst tw + 1) = snd tw' B (fst tw')"
-      using * unfolding \<open>next_time_world tw' = fst tw + 1\<close> by auto
-    moreover have "fst tw' = fst tw"
-      unfolding tw'_def by (simp add: worldline_upd2_def)
-    ultimately have "snd tw' A (fst tw + 1) = snd tw' A (fst tw)" and "snd tw' B (fst tw + 1) = snd tw' B (fst tw)"
-      by auto
-    have "snd tw' C (fst tw + 1) \<longleftrightarrow> \<not> (snd tw' A (fst tw) \<and> snd tw' B (fst tw))"
-      unfolding tw'_def worldline_upd2_def worldline_upd_def beval_world_raw2_def beval_world_raw_def
-      state_of_world_def beh_of_world_raw_def 
-      by auto
-    thus ?thesis
-      using \<open>snd tw' A (get_time tw + 1) = snd tw' A (get_time tw)\<close> \<open>snd tw' B (get_time tw + 1) =
-      snd tw' B (get_time tw)\<close> \<open>snd tw' C (get_time tw + 2) = snd tw' C (get_time tw + 1)\<close> by blast
-  qed
-  moreover have "\<forall>i> fst tw + 2. snd tw' C i = snd tw' C (fst tw + 2)"
-    unfolding tw'_def worldline_upd2_def worldline_upd_def by auto
-  ultimately show "snd (next_time_world tw', snd tw') C (get_time (next_time_world tw', snd tw') + 1) =
-    (\<not> (snd (next_time_world tw', snd tw') A (get_time (next_time_world tw', snd tw')) \<and>
-         snd (next_time_world tw', snd tw') B (get_time (next_time_world tw', snd tw')))) \<and>
-    (\<forall>i>get_time (next_time_world tw', snd tw') + 1.
-        snd (next_time_world tw', snd tw') C i = snd (next_time_world tw', snd tw') C (get_time (next_time_world tw', snd tw') + 1))"
-    by (simp add: \<open>next_time_world tw' = get_time tw + 1\<close>)
-qed
-
-lemma nand_seq_hoare_next_time3:
-  "\<turnstile> [\<lambda>tw. True] (Bassign_trans C (Bnand (Bsig A) (Bsig B)) 1) [\<lambda>tw. nand_inv3 (next_time_world tw, snd tw)]"
-  apply (rule Conseq2[where Q="\<lambda>tw. nand_inv3 (next_time_world tw, snd tw)", rotated 1], rule Assign2)
-  using nand_inv3_next_time by auto
-
-lemma disjnt_AB_eq:
-  "disjnt {A, B} s \<longleftrightarrow> (s = {} \<or> s = {C})"
-  by (rule, metis Diff_UNIV Diff_insert0 Diff_single_insert UNIV_sig disjnt_insert1 empty_subsetI
-  subset_singleton_iff) auto
-
-lemma nand_inv_next_time_disjnt1:
-  assumes "nand_inv tw" and "nand_inv2 tw"
-  assumes "event_of tw = {C}"
-  shows   "nand_inv (next_time_world tw, snd tw)"
-proof (cases "fst tw = 0")
-  case False
-  have "fst tw < next_time_world tw"
-    using next_time_world_at_least  using nat_less_le by blast
-  have *: "(\<forall>i> fst tw. snd tw C i = snd tw C (fst tw))"
-    using assms(2-3) unfolding nand_inv2_def by auto
-  have "\<forall>i < next_time_world tw. snd tw C (i + 1) \<longleftrightarrow> \<not> (snd tw A i \<and> snd tw B i)"
-  proof (rule allI, rule impI)
-    fix i
-    assume "i < next_time_world tw"
-    hence "i < fst tw \<or> fst tw \<le> i \<and> i \<le> next_time_world tw - 1"
-      using \<open>fst tw < next_time_world tw\<close> by linarith  
-    moreover
-    { assume "i < fst tw"
-      hence "snd tw C (i + 1) \<longleftrightarrow> \<not> (snd tw A i \<and> snd tw B i)"
-        using assms(1) unfolding nand_inv_def by auto }
-    moreover
-    { assume " fst tw \<le> i \<and> i \<le> next_time_world tw - 1"
-      hence "snd tw C (i + 1) \<longleftrightarrow> snd tw C (fst tw + 1)"
-        using unchanged_until_next_time_world "*" by force
-      also have "... \<longleftrightarrow> snd tw C (fst tw)"
-        using * by auto
-      also have "... \<longleftrightarrow> \<not> (snd tw A (fst tw - 1) \<and> snd tw B (fst tw - 1))"
-        using assms(1) False unfolding nand_inv_def 
-        by (metis Suc_eq_plus1 add.commute add_diff_inverse_nat lessI less_one)
-      finally have "snd tw C (i + 1) \<longleftrightarrow> \<not> (snd tw A (fst tw - 1) \<and> snd tw B (fst tw - 1))"
-        by auto
-      moreover have "snd tw A i \<longleftrightarrow> snd tw A (fst tw)" and "snd tw B i \<longleftrightarrow> snd tw B (fst tw)"
-        using unchanged_until_next_time_world \<open>fst tw \<le> i \<and> i \<le> next_time_world tw - 1\<close>
-        by (simp add: unchanged_until_next_time_world \<open>i < next_time_world tw\<close>)+
-      moreover have "(snd tw A (fst tw) \<longleftrightarrow> snd tw A (fst tw - 1)) \<and> (snd tw B (fst tw) \<longleftrightarrow> snd tw B (fst tw - 1))"
-      proof -
-        have "event_of tw = {s. snd tw s (fst tw) \<noteq> snd tw s (fst tw - 1)}"
-          using False unfolding event_of_alt_def by auto
-        with \<open>event_of tw = {C}\<close> have "snd tw A (fst tw) = snd tw A (fst tw - 1)" and 
-                                      "snd tw B (fst tw) = snd tw B (fst tw - 1)"
-          by auto
-        thus ?thesis
-          by auto
-      qed
-      ultimately have "snd tw A i \<longleftrightarrow> snd tw A (fst tw - 1)" and "snd tw B i \<longleftrightarrow> snd tw B (fst tw - 1)"
-        by auto
-      hence "snd tw C (i + 1) \<longleftrightarrow> \<not> (snd tw A i \<and> snd tw B i)"
-        using \<open>snd tw C (i + 1) = (\<not> (snd tw A (get_time tw - 1) \<and> snd tw B (get_time tw - 1)))\<close> by
-        blast }
-    ultimately show "snd tw C (i + 1) \<longleftrightarrow> \<not> (snd tw A i \<and> snd tw B i)"
-      by blast
-  qed
-  thus ?thesis
-    by (simp add: nand_inv_def)
-next
-  case True
-  hence *: "(\<forall>i. snd tw C i = snd tw C (fst tw))"
-    using assms(2-3) unfolding nand_inv2_def by (metis neq0_conv singletonI)  
-  have "0 < next_time_world tw"
-    using True next_time_world_at_least nat_less_le  by metis
-  have "\<forall>i < next_time_world tw. snd tw C (i + 1) \<longleftrightarrow> \<not> (snd tw A i \<and> snd tw B i)"
-  proof (rule allI, rule impI)
-    fix i
-    assume "i < next_time_world tw"
-    hence "snd tw C (i + 1) \<longleftrightarrow> snd tw C 1"
-      using unchanged_until_next_time_world "*" by blast
-    also have "... \<longleftrightarrow> snd tw C 0"
-      using * by auto
-    also have "... \<longleftrightarrow> \<not> (snd tw A 0 \<and> snd tw B 0)"
-    proof -
-      have "event_of tw = {s. snd tw s 0 \<noteq> False}"
-        unfolding event_of_alt_def True by auto
-      with \<open>event_of tw ={C}\<close> have "snd tw C 0 = True" and "snd tw A 0 = False" and "snd tw B 0 = False"
-        by auto
-      thus ?thesis
-        by auto
-    qed
-    finally have "snd tw C (i + 1) \<longleftrightarrow> \<not> (snd tw A 0 \<and> snd tw B 0)"
-      by auto
-    moreover have "snd tw A i \<longleftrightarrow> snd tw A 0" and "snd tw B i \<longleftrightarrow> snd tw B 0"
-      using unchanged_until_next_time_world 
-      by (simp add: unchanged_until_next_time_world True \<open>i < next_time_world tw\<close>)+
-    hence "snd tw C (i + 1) \<longleftrightarrow> \<not> (snd tw A i \<and> snd tw B i)"
-      using calculation by blast
-    ultimately show "snd tw C (i + 1) \<longleftrightarrow> \<not> (snd tw A i \<and> snd tw B i)"
-      by blast
-  qed
-  thus ?thesis
-    by (simp add: nand_inv_def)
-qed
-
-lemma nand_inv_next_time_disjnt2:
-  assumes "nand_inv tw" and "nand_inv3 tw"
-  assumes "event_of tw = {}"
-  shows   "nand_inv (next_time_world tw, snd tw)"
-proof (cases "fst tw = 0")
-  case False
-  have "fst tw < next_time_world tw"
-    using next_time_world_at_least  using nat_less_le by blast
-  have **: "snd tw C (fst tw + 1) \<longleftrightarrow> \<not> (snd tw A (fst tw) \<and> snd tw B (fst tw))"
-    using assms(2-3) unfolding nand_inv3_def by auto
-  have *: "\<forall>i> fst tw + 1. snd tw C i = snd tw C (fst tw + 1)"
-    using assms(2-3) unfolding nand_inv3_def by auto
-  have "\<forall>i < next_time_world tw. snd tw C (i + 1) \<longleftrightarrow> \<not> (snd tw A i \<and> snd tw B i)"
-  proof (rule allI, rule impI)
-    fix i
-    assume "i < next_time_world tw"
-    hence "i < fst tw \<or> fst tw \<le> i \<and> i \<le> next_time_world tw - 1"
-      using \<open>fst tw < next_time_world tw\<close> by linarith  
-    moreover
-    { assume "i < fst tw"
-      hence "snd tw C (i + 1) \<longleftrightarrow> \<not> (snd tw A i \<and> snd tw B i)"
-        using assms(1) unfolding nand_inv_def by auto }
-    moreover
-    { assume " fst tw \<le> i \<and> i \<le> next_time_world tw - 1"
-      hence "snd tw C (i + 1) \<longleftrightarrow> snd tw C (fst tw + 1)"
-        using unchanged_until_next_time_world "*"  using nat_less_le by auto
-      moreover have "snd tw A i \<longleftrightarrow> snd tw A (fst tw)" and "snd tw B i \<longleftrightarrow> snd tw B (fst tw)"
-        using unchanged_until_next_time_world \<open>fst tw \<le> i \<and> i \<le> next_time_world tw - 1\<close>
-        by (simp add: unchanged_until_next_time_world \<open>i < next_time_world tw\<close>)+
-      ultimately have "snd tw C (i + 1) \<longleftrightarrow> \<not> (snd tw A i \<and> snd tw B i)"
-        using ** by auto }
-    ultimately show "snd tw C (i + 1) \<longleftrightarrow> \<not> (snd tw A i \<and> snd tw B i)"
-      by blast
-  qed
-  thus ?thesis
-    by (simp add: nand_inv_def)  
-next
-  case True
-  have **: "snd tw C (fst tw + 1) \<longleftrightarrow> \<not> (snd tw A (fst tw) \<and> snd tw B (fst tw))"
-    using assms(2-3) True unfolding nand_inv3_def by auto
-  have "\<forall>i> fst tw + 1. snd tw C i = snd tw C (fst tw + 1)"
-    using assms(2-3) unfolding nand_inv3_def by auto
-  hence *: "\<forall>i>1. snd tw C i = snd tw C 1"
-    using True by auto
-  have "0 < next_time_world tw"
-    using True next_time_world_at_least nat_less_le  by metis
-  have "\<forall>i < next_time_world tw. snd tw C (i + 1) \<longleftrightarrow> \<not> (snd tw A i \<and> snd tw B i)"
-  proof (rule allI, rule impI)
-    fix i
-    assume "i < next_time_world tw"
-    hence "snd tw C (i + 1) \<longleftrightarrow> snd tw C 1"
-      using "*"   by (metis One_nat_def Suc_eq_plus1 less_add_same_cancel2 neq0_conv)
-    also have "... \<longleftrightarrow> \<not> (snd tw A 0 \<and> snd tw B 0)"
-      using "**" True by auto
-    finally have "snd tw C (i + 1) \<longleftrightarrow> \<not> (snd tw A 0 \<and> snd tw B 0)"
-      by auto
-    moreover have "snd tw A i \<longleftrightarrow> snd tw A 0" and "snd tw B i \<longleftrightarrow> snd tw B 0"
-      using unchanged_until_next_time_world 
-      by (simp add: unchanged_until_next_time_world True \<open>i < next_time_world tw\<close>)+
-    hence "snd tw C (i + 1) \<longleftrightarrow> \<not> (snd tw A i \<and> snd tw B i)"
-      using calculation by blast
-    ultimately show "snd tw C (i + 1) \<longleftrightarrow> \<not> (snd tw A i \<and> snd tw B i)"
-      by blast
-  qed
-  thus ?thesis
-    by (simp add: nand_inv_def)
-qed
-
-lemma nand_inv_123_next_time:
-  "\<forall>tw. (nand_inv tw \<and> nand_inv2 tw \<and> nand_inv3 tw) \<and> disjnt {A, B} (event_of tw) \<longrightarrow>
-         nand_inv (next_time_world tw, snd tw) \<and> nand_inv2 (next_time_world tw, snd tw) \<and> nand_inv3 (next_time_world tw, snd tw)"
-proof (rule allI, rule impI)
-  fix tw
-  assume "(nand_inv tw \<and> nand_inv2 tw \<and> nand_inv3 tw) \<and> disjnt {A, B} (event_of tw)"
-  hence "nand_inv tw" and "nand_inv2 tw" and "nand_inv3 tw" and "disjnt {A, B} (event_of tw)"
-    by auto
-  hence "event_of tw = {} \<or> event_of tw = {C}"
-    unfolding disjnt_AB_eq by auto
-  moreover
-  { assume "event_of tw = {C}"
-    with \<open>nand_inv tw\<close> and \<open>nand_inv2 tw\<close> have "nand_inv (next_time_world tw, snd tw)"
-      using nand_inv_next_time_disjnt1 by auto
-    moreover have "nand_inv2 (next_time_world tw, snd tw)"
-      using \<open>nand_inv2 tw\<close> next_time_world_at_least \<open>event_of tw ={C}\<close>
-      unfolding nand_inv2_def  by (metis dual_order.strict_trans fst_eqD singletonI snd_eqD)
-    moreover have "nand_inv3 (next_time_world tw, snd tw)"
-    proof -
-      { assume " event_of (next_time_world tw, snd tw) = {}"
-        hence "snd tw A (next_time_world tw) = snd tw A (next_time_world tw - 1)" and 
-              "snd tw B (next_time_world tw) = snd tw B (next_time_world tw - 1)"
-          unfolding event_of_alt_def
-          by (smt \<open>event_of (next_time_world tw, snd tw) = {}\<close> empty_Collect_eq event_of_alt_def
-                  fst_conv next_time_world_at_least not_less0 snd_conv)+
-        moreover have "snd tw C (next_time_world tw + 1) = snd tw C (next_time_world tw)"
-          by (metis (mono_tags, hide_lams) \<open>event_of tw = {C}\<close> \<open>nand_inv2 tw\<close> discrete insertI1
-              nand_inv2_def nat_less_le next_time_world_at_least not_less)
-        moreover have "snd tw C (next_time_world tw) \<longleftrightarrow> 
-                    \<not> (snd tw A (next_time_world tw - 1) \<and> snd tw B (next_time_world tw - 1))"
-          using \<open>nand_inv (next_time_world tw, snd tw)\<close> unfolding nand_inv_def
-          by (metis Suc_diff_1 diff_is_0_eq' diff_less fst_conv le_add_diff_inverse2 nat_less_le
-              next_time_world_at_least not_less not_less0 snd_conv zero_less_one)
-        ultimately have "snd tw C (next_time_world tw + 1) \<longleftrightarrow> 
-                        \<not> (snd tw A (next_time_world tw) \<and> snd tw B (next_time_world tw))" (is "?po1")
-          by blast
-        have "\<forall>i>next_time_world tw + 1. snd tw C i = snd tw C (next_time_world tw + 1)" (is "?po2")
-          using \<open>nand_inv2 (next_time_world tw, snd tw)\<close> \<open>event_of tw ={C}\<close> unfolding nand_inv2_def
-          by (metis (no_types, hide_lams) \<open>nand_inv2 tw\<close> dual_order.strict_trans insertI1 less_add_one
-          nand_inv2_def next_time_world_at_least)
-        with \<open>?po1\<close> have "?po1 \<and> ?po2"
-          by auto }
-      thus ?thesis
-        unfolding nand_inv3_def by auto
-    qed
-    ultimately have "nand_inv (next_time_world tw, snd tw) \<and> nand_inv2 (next_time_world tw, snd tw)
-                    \<and> nand_inv3 (next_time_world tw, snd tw)"
-      by auto }
-  moreover
-  { assume "event_of tw = {}"
-    with \<open>nand_inv tw\<close> and \<open>nand_inv3 tw\<close> have "nand_inv (next_time_world tw, snd tw)"
-      using nand_inv_next_time_disjnt2 by auto
-    moreover have "nand_inv2 (next_time_world tw, snd tw)"
-    proof -
-      { assume " C \<in> event_of (next_time_world tw, snd tw)"
-        have "(\<forall>i>get_time tw + 1. snd tw C i = snd tw C (get_time tw + 1))"
-          using \<open>nand_inv3 tw\<close> \<open>event_of tw = {}\<close>  unfolding nand_inv3_def
-          by auto
-        hence "\<forall>i>next_time_world tw. snd tw C i = snd tw C (next_time_world tw)"
-          using next_time_world_at_least 
-          by (smt discrete le_neq_implies_less less_imp_le less_le_trans) }
-      thus ?thesis
-        unfolding nand_inv2_def by auto
-    qed
-    moreover have "nand_inv3 (next_time_world tw, snd tw)"
-    proof -
-      { assume "event_of (next_time_world tw, snd tw) = {}"
-        with \<open>event_of tw = {}\<close> have "next_time_world tw = fst tw + 1" (is "?ntime")
-          using successive_empty_event  by blast
-        hence "snd tw C (fst tw + 2) \<longleftrightarrow> snd tw C (fst tw + 1)"
-          using \<open>event_of (next_time_world tw, snd tw) = {}\<close> unfolding event_of_alt_def
-          by (metis (no_types, lifting) Suc_eq_plus1 \<open>event_of tw = {}\<close> \<open>nand_inv3 tw\<close> add_Suc_right
-          lessI nand_inv3_def one_add_one)
-        have "snd tw C (fst tw + 1) \<longleftrightarrow> \<not> (snd tw A (fst tw) \<and> snd tw B (fst tw))"
-          using \<open>nand_inv (next_time_world tw, snd tw)\<close> unfolding \<open>next_time_world tw = fst tw + 1\<close>
-          nand_inv_def by auto
-        moreover have "snd tw A (fst tw) = snd tw A (fst tw + 1)" and "snd tw B (fst tw) = snd tw B (fst tw + 1)"
-          using \<open>event_of (next_time_world tw, snd tw) = {}\<close> \<open>next_time_world tw = get_time tw + 1\<close> event_of_alt_def 
-          by fastforce+
-        ultimately have "snd tw C (fst tw + 2) \<longleftrightarrow> \<not> (snd tw A (fst tw + 1) \<and> snd tw B (fst tw + 1))" (is "?po1")
-          using \<open>snd tw C (get_time tw + 2) = snd tw C (get_time tw + 1)\<close> by blast
-        have "\<forall>i>next_time_world tw + 1. snd tw C i = snd tw C (next_time_world tw+ 1)" (is "?po2")
-          using \<open>nand_inv3 tw\<close> \<open>event_of tw = {}\<close> 
-          unfolding \<open>next_time_world tw = fst tw + 1\<close>  nand_inv3_def by auto
-        with \<open>?po1\<close> \<open>?ntime\<close> have "?po1 \<and> ?po2 \<and> ?ntime"
-          by auto }
-      thus ?thesis
-        unfolding nand_inv3_def by auto
-    qed
-    ultimately have "nand_inv (next_time_world tw, snd tw) \<and> nand_inv2 (next_time_world tw, snd tw)
-                    \<and> nand_inv3 (next_time_world tw, snd tw)"
-      by auto }
-  ultimately show "nand_inv (next_time_world tw, snd tw) \<and> nand_inv2 (next_time_world tw, snd tw)
-                    \<and> nand_inv3 (next_time_world tw, snd tw)"
-    by auto
-qed
-
-lemma nand_conc_hoare:
-  "\<turnstile> \<lbrace>\<lambda>tw. nand_inv tw \<and> nand_inv2 tw \<and> nand_inv3 tw\<rbrace> nand3 \<lbrace>\<lambda>tw. nand_inv  (next_time_world tw, snd tw) \<and> 
-                                                                  nand_inv2 (next_time_world tw, snd tw) \<and> 
-                                                                  nand_inv3 (next_time_world tw, snd tw)\<rbrace>"
+  
+lemma nand_conc_hoare3:
+  "\<turnstile> \<lbrace>\<lambda>tw. nand_inv tw \<and> nand_inv2 tw\<rbrace> nand3 \<lbrace>\<lambda>tw. nand_inv  (next_time_world tw, snd tw)  \<and> nand_inv2  (next_time_world tw, snd tw)\<rbrace>"
   unfolding nand3_def
   apply (rule Single)
+   apply (unfold conj_assoc)
    apply (rule compositional_conj)
-    apply (rule strengthen_precondition)
     apply(rule nand_seq_hoare_next_time)
-   apply(rule Conj)
-    apply(rule Conseq2[where P="\<lambda>tw. True"])
-      apply simp
-     apply(rule nand_seq_hoare_next_time2)
-    apply simp
+   apply (rule strengthen_precondition)
    apply(rule Conseq2[where P="\<lambda>tw. True"])
      apply simp
-     apply(rule nand_seq_hoare_next_time3)
+    apply (rule nand_seq_hoare_next_time4)
    apply simp
-  apply (rule nand_inv_123_next_time)
+  apply (rule allI)
+  apply (rule impI)
+  apply (rule conjI)
+   apply (erule nand_conc_hoare')
+  apply (erule nand_conc_hoare2)
   done
 
-lemma nand_conc_sim:
-  "\<turnstile>\<^sub>s \<lbrace>\<lambda>tw. nand_inv tw \<and> nand_inv2 tw \<and> nand_inv3 tw\<rbrace> nand3 \<lbrace>\<lambda>tw. nand_inv tw \<and> nand_inv2 tw \<and> nand_inv3 tw\<rbrace>"
+lemma nand_conc_sim':
+  "\<turnstile>\<^sub>s \<lbrace>\<lambda>tw. nand_inv tw \<and> nand_inv2 tw\<rbrace> nand3 \<lbrace>\<lambda>tw. nand_inv tw \<and> nand_inv2 tw\<rbrace>"
   apply (rule While)
-  apply (rule nand_conc_hoare)
+  apply (rule nand_conc_hoare3)
   done
 
-lemma nand_conc_sim2:
-  "\<turnstile>\<^sub>s \<lbrace>\<lambda>tw. nand_inv tw \<and> nand_inv2 tw \<and> nand_inv3 tw\<rbrace> nand3 \<lbrace>nand_inv\<rbrace>"
-  by (rule Conseq_sim[where Q="\<lambda>tw. nand_inv tw \<and> nand_inv2 tw \<and> nand_inv3 tw" and 
-                            P="\<lambda>tw. nand_inv tw \<and> nand_inv2 tw \<and> nand_inv3 tw"])
-     (simp_all add: nand_conc_sim)
+lemma nand_conc_sim2':
+  "\<turnstile>\<^sub>s \<lbrace>\<lambda>tw. nand_inv tw \<and> nand_inv2 tw\<rbrace> nand3 \<lbrace>nand_inv\<rbrace>"
+  by (rule Conseq_sim[where Q="\<lambda>tw. nand_inv tw \<and> nand_inv2 tw" and 
+                            P="\<lambda>tw. nand_inv tw \<and> nand_inv2 tw"])
+     (simp_all add: nand_conc_sim')  
 
 text \<open>Initialisation preserves the invariant\<close>
 
@@ -544,31 +309,20 @@ lemma init_sat_nand_inv:
   apply (rule nand_seq_hoare_next_time0)
   done
 
-lemma init_sat_nand_inv2:
+lemma init_sat_nand_inv2: 
   "init_sim_hoare (\<lambda>tw. True) nand3 nand_inv2"
   unfolding nand3_def
   apply (rule AssignI)
   apply (rule SingleI)
-  apply (rule nand_seq_hoare_next_time2)
-  done
-
-lemma init_sat_nand_inv3:
-  "init_sim_hoare (\<lambda>tw. True) nand3 nand_inv3"
-  unfolding nand3_def
-  apply (rule AssignI)
-  apply (rule SingleI)
-  apply (rule nand_seq_hoare_next_time3)
+  apply (rule nand_seq_hoare_next_time4)
   done
 
 lemma init_sat_nand_inv_comb:
-  "init_sim_hoare (\<lambda>tw. fst tw = 0) nand3 (\<lambda>tw. nand_inv tw \<and> nand_inv2 tw \<and> nand_inv3 tw)"
+  "init_sim_hoare (\<lambda>tw. fst tw = 0) nand3 (\<lambda>tw. nand_inv tw \<and> nand_inv2 tw)"
   apply (rule ConjI_sim)
   apply (rule init_sat_nand_inv)
-  apply (rule ConjI_sim)
   apply (rule ConseqI_sim[where P="\<lambda>tw. True" and Q="nand_inv2"])
   apply (simp, rule init_sat_nand_inv2, simp)
-  apply (rule ConseqI_sim[where P="\<lambda>tw. True" and Q="nand_inv3"])
-  apply (simp, rule init_sat_nand_inv3, simp)
   done
 
 lemma nand_correctness:
@@ -583,13 +337,13 @@ proof -
     unfolding conc_stmt_wf_def nand3_def by auto
   moreover have "nonneg_delay_conc nand3"
     unfolding nand3_def by auto
-  ultimately have "init_sim_valid (\<lambda>tw. fst tw = 0) nand3 (\<lambda>tw. nand_inv tw \<and> nand_inv2 tw \<and> nand_inv3 tw)"
+  ultimately have "init_sim_valid (\<lambda>tw. fst tw = 0) nand3 (\<lambda>tw. nand_inv tw \<and> nand_inv2 tw)"
     using init_sim_hoare_soundness[OF init_sat_nand_inv_comb] by auto
-  hence "nand_inv tw" and "nand_inv2 tw" and "nand_inv3 tw"
+  hence "nand_inv tw" and "nand_inv2 tw"
     using \<open>init_sim (0, w) nand3 = tw\<close> fst_conv unfolding init_sim_valid_def 
     by fastforce+ 
-  moreover have "\<Turnstile>\<^sub>s \<lbrace>\<lambda>tw. nand_inv tw \<and> nand_inv2 tw \<and> nand_inv3 tw\<rbrace> nand3 \<lbrace>nand_inv\<rbrace>"
-    using conc_sim_soundness[OF nand_conc_sim2] \<open>conc_stmt_wf nand3\<close> \<open>nonneg_delay_conc nand3\<close>
+  moreover have "\<Turnstile>\<^sub>s \<lbrace>\<lambda>tw. nand_inv tw \<and> nand_inv2 tw\<rbrace> nand3 \<lbrace>nand_inv\<rbrace>"
+    using conc_sim_soundness[OF nand_conc_sim2'] \<open>conc_stmt_wf nand3\<close> \<open>nonneg_delay_conc nand3\<close>
     by auto
   ultimately have "nand_inv tw'"
     using \<open>tw, i + 1, nand3 \<Rightarrow>\<^sub>S tw'\<close> unfolding sim_hoare_valid_def by blast
@@ -598,6 +352,5 @@ proof -
   with \<open>i + 1 < fst tw'\<close> show ?thesis
     by auto
 qed
-
-                
+     
 end
